extraction/theories/Utils.v
@@ -161,7 +161,7 @@ Definition kername_set_of_list (l : list kername) : KernameSet.t :=
   fold_left (fun s k => KernameSet.add k s) l KernameSet.empty.
 
 (* When extracting this can be remapped as something that measures and outputs some info *)
-Definition timed {A} (part : string) (f : unit -> A) : A :=
+Definition timed {A} (part : String.string) (f : unit -> A) : A :=
   f tt.
 
 Arguments timed /.
